Some updates

theories/examples/las.v
@@ -15,31 +15,42 @@ Section las_example.
   (* [promotable] is the register that will be analyzed for load after store
      [stored_value] is the current register whose value is stored in the address
       at [promotable]. *)
- Definition las_instr {A : Set} {T}
-   (promotable : raw_id) (stored_val : option raw_id) (i : A * instr T) :=
-    match i with
-    (* A load instruction from a stored [raw_id] that hasn't been modified. *)
-    | (promotable_id, INSTR_Load _ _ (_, EXP_Ident (ID_Local ptr)) _) =>
-      if decide (promotable = ptr) then
-        match stored_val with
-          | Some c =>
-              (* The promotable location has been written to; substitute the load
-                 for the local identifier for the promotable location instead. *)
-              ((promotable_id, INSTR_Op (EXP_Ident (ID_Local promotable))), stored_val)
-          | None => (i, stored_val)
-        end
-      else (i, stored_val)
-    (* A store instruction to the promoted local identifier. *)
-    | (_, INSTR_Store _
-              (_, EXP_Ident (ID_Local v'))
-              (_, EXP_Ident (ID_Local ptr)) _) =>
+ Definition las_instr {T}
+   (promotable : raw_id) (stored_val : option raw_id) (i : _ * instr T) (allocated : bool) :=
+    if allocated then
+      match i with
+      (* A load instruction from a stored [raw_id] that hasn't been modified. *)
+      | (IId promotable_id, INSTR_Load _ _ (_, EXP_Ident (ID_Local ptr)) _) =>
         if decide (promotable = ptr) then
-          (* Update the stored value *)
-          (i, Some v')
-        else
-          (i, stored_val)
-    | x => (i, stored_val)
-    end.
+          match stored_val with
+            | Some c =>
+                (* The promotable location has been written to; substitute the load
+                  for the local identifier for the promotable location instead. *)
+                ((IId promotable_id, INSTR_Op (EXP_Ident (ID_Local c))), stored_val, allocated)
+            | None => (i, stored_val, allocated)
+          end
+        else (i, stored_val, allocated)
+      (* A store instruction to the promoted local identifier. *)
+      | (IVoid _, INSTR_Store _
+                (_, EXP_Ident (ID_Local v'))
+                (_, EXP_Ident (ID_Local ptr)) _) =>
+          if decide (promotable = ptr) then
+            (* Update the stored value *)
+            (i, Some v', allocated)
+          else
+            (i, stored_val, allocated)
+      | x => (i, stored_val, allocated)
+      end
+    else
+      match i with
+      (* The alloca instruction with promotable id. *)
+      | (IId id, INSTR_Alloca _ _ _) =>
+        if decide (promotable = id)
+        then (i, stored_val, true)
+        else (i, stored_val, allocated)
+      | _ => (i, stored_val, allocated)
+      end
+   .
 
   (* Given a code block [c] and a promotable location, (i.e. a local identifier
      that stores a non-aliased location that has been allocated in the current block),
@@ -54,14 +65,14 @@ Section las_example.
       - Figure out if there is a normal form that can be enforced to make
                 sure expressions refer to [local_id]s. *)
   Fixpoint las_code {T}
-    (promotable : local_id) (stored_val : option raw_id) (c : code T) :=
+    (promotable : local_id) (stored_val : option raw_id) (c : code T) (allocated : bool) :=
     match c with
     | nil => nil
     | x :: tl =>
-        let '(x, v) :=
-          las_instr promotable stored_val x
+        let '(x, v, allocated) :=
+          las_instr promotable stored_val x allocated
         in
-        x :: las_code promotable v tl
+        x :: las_code promotable v tl allocated
     end.
 
   Definition las_block {T} (a : raw_id) (v : option raw_id) (b : LLVMAst.block T) :
@@ -69,7 +80,7 @@ Section las_example.
       mk_block
         (blk_id b)
         (blk_phis b)
-        (las_code a v (blk_code b))
+        (las_code a v (blk_code b) false)
         (blk_term b)
         (blk_comments b).
 
@@ -113,6 +124,10 @@ Section las_example.
         expr_contains_raw_id e1 i || expr_contains_raw_id e2 i
     | _ => false
     end.
+
+  Definition phi_contains_raw_id {T} (e : phi T) (i : raw_id) : bool :=
+    let '(Phi t l) := e in
+    List.existsb (fun x => expr_contains_raw_id x.2 i) l.
 
   (* FUTURE WORK: Alias analysis *)
   Definition promotable_instr {T} (i : instr_id * instr T) a : bool :=
@@ -171,7 +186,7 @@ Example code1 : code dtyp :=
                   (DTYPE_I 32, EXP_Ident (ID_Local (Name "b")))
                   (DTYPE_Pointer, EXP_Ident (ID_Local (Name "a")))
                    None) ::
-  (IId (Name "b"), INSTR_Load true (DTYPE_I 32)
+  (IId (Name "c"), INSTR_Load true (DTYPE_I 32)
       (DTYPE_I 32, EXP_Ident (ID_Local (Name "a"))) None) ::
   nil.
 
@@ -194,7 +209,7 @@ Example cfg1 : cfg dtyp :=
 Compute (find_promotable_alloca cfg1).
 
 Compute (las cfg1).
-Compute (las_code (Name "a") None code1).
+Compute (las_code (Name "a") None code1 false).
 
 (* ------------------------------------------------------------------- *)
 (* Specification of the Load-after-store optimization. *)
@@ -214,39 +229,105 @@ From velliris.vir Require Import logical_relations tactics.
 (* ------------------------------------------------------------------- *)
 
 (* TODO: Move and prove on [wellformedness]. *)
+
+(* LATER: FIXME Unify [is_true] and [Is_true] coercion *)
 Lemma fun_WF_inv f:
-  fun_WF f -> cfg_WF (df_instrs f).
-Proof. Admitted.
+  fun_WF f ->
+  NoDup (df_args f) /\ cfg_WF (df_instrs f).
+Proof.
+  rewrite /fun_WF; intros WF; destructb; split;
+    [ apply NoDup_b_NoDup1 ; by rewrite H | done ].
+Qed.
 
 (* TODO: Move *)
 Lemma cfg_WF_inv f:
   cfg_WF f ->
   ocfg_WF (blks f).
-Proof. Admitted.
+Proof. done. Qed.
 
+(* ------------------------------------------------------------------- *)
+Ltac splitb :=
+  repeat match goal with
+  | |- is_true (_ && _) =>
+      apply Bool.andb_true_iff; split
+  | |- Is_true (_ && _) =>
+      apply andb_True; split
+  end.
+
+(* TODO : Write subcases for all [WF] constructs *)
+Ltac invert_WF :=
+  match goal with
+    | [ H : is_true (block_WF _) |- _ ] =>
+        let WF_code := fresh "WF_code" in
+        let WF_term := fresh "WF_term" in
+        apply block_WF_inv in H;
+        destruct H as (WF_code & WF_term)
+    | [ H : is_true (fun_WF _) |- _ ] =>
+        let WF_args := fresh "WF_args" in
+        let WF_cfg := fresh "WF_cfg" in
+        apply fun_WF_inv in H;
+        destruct H as (WF_args & WF_cfg)
+  end.
 (* ------------------------------------------------------------------- *)
 (* Well-formedness is preserved in the LAS transformation. *)
 
-Lemma las_block_WF a0 a s:
-  block_WF a ->
-  block_WF (las_block a0 s a).
-Proof. Admitted.
+Lemma las_instr_WF:
+  ∀ (a : instr_id * instr dtyp) (p : local_id) (v : option raw_id)
+    (bi bf : bool) (id : instr_id) (instr : instr dtyp) (o : option raw_id),
+  instr_WF a.2 ->
+  las_instr p v a bi = (id, instr, o, bf) →
+  instr_WF instr.
+Proof.
+  intros * WF Hinstr.
+  rewrite /las_instr in Hinstr.
+  destruct_if; by destruct_match.
+Qed.
 
-Lemma las_code_WF a0 a s:
-  code_WF a0 ->
-  code_WF (las_code a s a0).
-Proof. Admitted.
+Lemma las_code_WF p v c b:
+  code_WF c ->
+  code_WF (las_code p v c b).
+Proof.
+  intros WF; revert p v b.
+  induction c; first done.
+  destruct (code_WF_cons_inv _ _ WF) as (WF_i & WF_c).
+  specialize (IHc WF_c).
+  intros *; cbn.
+  destruct (las_instr p v a b) as (((?&?)&?)&?)
+    eqn: Hinstr; cbn.
+  splitb; [ by eapply las_instr_WF | apply IHc ].
+Qed.
 
-Lemma las_fun_WF f:
-  fun_WF f ->
-  fun_WF (las_fun f).
-Proof. Admitted.
+Lemma las_block_WF p v b:
+  block_WF b ->
+  block_WF (las_block p v b).
+Proof.
+  intros WF; invert_WF.
+  apply (las_code_WF p v _ false) in WF_code.
+  rewrite /block_WF; by splitb.
+Qed.
 
 Lemma las_ocfg_WF f a:
   ocfg_WF f ->
   ocfg_WF (las_ocfg a f).
 Proof.
   intros. induction f; eauto.
+Admitted.
+
+(* TODO *)
+Ltac reflectb :=
+  repeat match goal with
+  | [ H : NoDup_b _ = true |- _] => apply NoDup_b_NoDup in H
+  | [ H : Nat.eqb _ _ = true |- _] => apply Nat.eqb_eq in H
+  | [ H : forallb _ _ = true |- _] => rewrite forallb_True in H
+  end.
+
+Lemma las_fun_WF f:
+  fun_WF f ->
+  fun_WF (las_fun f).
+Proof.
+  intros WF. invert_WF.
+  rewrite /fun_WF; splitb.
+
 Admitted.
 
 Lemma las_cfg_WF f:
@@ -267,6 +348,42 @@ Qed.
 
 (* ------------------------------------------------------------------- *)
 
+Lemma find_promotable_alloca_some {T} f promotable instr:
+  find_promotable_alloca f = Some (IId promotable, instr) ->
+  let instrs := concat (map (blk_code (T := T)) (blks f)) in
+  (IId promotable) ∈ instrs.*1.
+Proof. Admitted.
+
+(* SSA definitions *)
+
+(* TODO: Move ? *)
+Definition SSA_cfg {T} (c : cfg T) :=
+  let ocfg := blks c in
+  let code := concat (map (blk_code (T := T)) ocfg) in
+  let code_ids : list raw_id :=
+    fold_left
+      (fun acc x =>
+          match x with
+          | IId i => i :: acc
+          | _ => acc
+          end)
+      code.*1 [] in
+  let phis :=
+    concat (map (blk_phis (T := T)) ocfg) in
+  (* The code ids and phi ids are disjoint *)
+  code_ids ## phis.*1 /\ NoDup code_ids /\ NoDup phis.*1.
+
+Definition SSA_function (f : function) :=
+  SSA_cfg (df_instrs f).
+
+Lemma SSA_fun_implies_promotable_phi_disjoint f instr promotable:
+  find_promotable_alloca f = Some (IId promotable, instr) ->
+  ∀ b : LLVMAst.block dtyp,
+    b ∈ blks f → (blk_phis b).*1 ## promotable :: nil.
+Proof. Admitted.
+
+(* ------------------------------------------------------------------- *)
+
 Section las_example_proof.
 
   Context `{vellirisGS Σ}.
@@ -274,20 +391,33 @@ Section las_example_proof.
   (* ------------------------------------------------------------------- *)
 
   (* TODO: Get from [fundamental.v] *)
-  Theorem fun_logrel_refl f:
+  Theorem expr_logrel_refl dt e C A_t A_s :
+    (⊢ expr_logrel local_bij alloca_bij C dt dt e e A_t A_s)%I.
+  Proof. Admitted.
+
+  Theorem instr_logrel_refl id e A_t A_s i_t i_s:
+    instr_WF e ->
+    (⊢ instr_logrel local_bij alloca_bij i_t i_s id e id e ∅ A_t A_s)%I.
+  Proof with vsimp. Admitted.
+
+  Theorem fun_logrel_refl f attr:
     fun_WF f ->
-    (⊢ fun_logrel f f ∅)%I.
+    (⊢ fun_logrel attr_inv attr f f ∅)%I.
   Proof. Admitted.
 
-  Definition local_bij_except_promotable promotable i_t i_s L_t L_s :=
-    (local_bij_except [promotable] [promotable] i_t i_s L_t L_s ∗
-    (⌜promotable ∈ L_t.*1⌝ -∗ ∃ v_t : local_val, [ promotable := v_t ]t i_t) ∗
-    (⌜promotable ∈ L_s.*1⌝ -∗ ∃ v_s : local_val, [ promotable := v_s ]s i_s))%I.
+  Theorem term_logrel_refl ϒ C:
+    (⊢ term_logrel local_bij alloca_bij ϒ ϒ C)%I.
+  Proof with vsimp. Admitted.
 
-  Lemma local_bij_implies_local_bij_except_promotable i_t i_s L_t L_s promotable:
-    local_bij i_t i_s L_t L_s -∗
-    local_bij_except_promotable promotable i_t i_s L_t L_s.
-  Proof. Admitted.
+  Theorem phis_compat ΠA C bid Φ Φ' A_t A_s l_t l_s:
+    Φ.*1 ## l_t ->
+    Φ'.*1 ## l_s ->
+    Φ.*1 = Φ'.*1 ->
+    ([∗ list] ϕ;ϕ' ∈ Φ; Φ',
+       phi_logrel local_bij
+         ΠA bid bid ϕ ϕ' C A_t A_s) -∗
+    phis_logrel local_bij ΠA bid bid Φ Φ' C A_t A_s.
+  Proof with vsimp. Admitted.
 
   Opaque find_promotable_alloca.
 
@@ -297,88 +427,122 @@ Section las_example_proof.
      trying to perform the optimization, thus we have the ownership for the
      locations. *)
 
-  (* [LAS] case where the load is removed. *)
-  (* FIXME: Use simulation relation directly *)
-  Lemma las_instr_sim_load
-    promotable v_t v_s i_t i_s ptr ptr' A_t A_s id val align b τ τ' l_t l_s:
-    let '((id', i'), v) :=
-      (las_instr promotable (Some val)
-         (IId id, INSTR_Load b τ (τ', EXP_Ident (ID_Local promotable)) align)) in
-    (* The promotable local id stores a pointer that is allocated on both source
-       and target. *)
-    [ id := l_s ]s i_s -∗
-    [ id := l_t ]t i_t -∗
-    [ promotable := UVALUE_Addr (ptr, 0%Z) ]s i_s -∗
-    ptr ↦s v_s  -∗
-    [ promotable := UVALUE_Addr (ptr', 0%Z) ]t i_t -∗
-    ptr ↦t v_t  -∗
-    dval_rel v_t v_s -∗
-    instr_logrel
-      (local_bij_except [promotable] [promotable])
-      alloca_bij
-      i_t i_s
-      id'
-      i'
-      (IId id)
-      (INSTR_Load b τ (τ', EXP_Ident (ID_Local promotable)) align)
-      ∅ A_t A_s.
-  Proof.
-    cbn; destruct_if_goal; try done.  clear e H0 H2.
-    (* Reduced *)
-    iIntros "Hids Hidt Hls Hps Hlt Hpt #Hv CI".
-    iApply target_red_sim_expr.
-    destruct_code_inv_all; repeat destruct_frame.
-    iApply (target_instr_local_write1 with "Hs_t Hd_t Hidt [Hlt]");
-      cycle 1; eauto.
-    { iIntros "Hid Hdt_t Hs_t".
-      rewrite /denote_instr_exp; cbn -[denote_op].
-      iApply target_red_eq_itree.
-      { by rewrite eq_itree_exp_conv_to_instr. }
-      iApply (target_local_id with "Hs_t Hlt").
-      iIntros "Hs_t Ht"; sfinal. }
-    iIntros "Ht Hd_t Hs_t".
-
-    iApply source_red_sim_expr.
-    iApply (source_instr_load with "Hps Hls Hd_s Hs_s"); last first.
-    (* Hd_s Hids [Hls]"); cycle 1; eauto. *)
-    { iIntros "Hid Hdt_t Hs_t' Hd_s Hs_s".
-      Base. do 2 sfinal.
-      iFrame "WF_frame".
-  Admitted.
-
   Lemma las_simulation_code a b A_t A_s :
     code_WF (blk_code b) ->
     ⊢ code_logrel
-        (local_bij_except_promotable a)
+        local_bij
         alloca_bij
         (blk_code (las_block a None b))
         (blk_code b)
         ∅ A_t A_s.
+  Local Ltac las_trivial Hlas :=
+    cbn in *; destruct_match; inv Hlas; destruct_if;
+    iIntros; try iApply instr_logrel_refl;
+    try by destructb.
   Proof.
     iIntros (?); iApply code_compat; eauto;
       first by apply las_code_WF.
+    remember None. clear Heqo.
+    cbn; remember (blk_code b); clear b Heqc.
+    remember false.
 
-    (* TODO: MEDIUM
-        [las_instr custom logical relation]. *)
+    (* TODO: Refactor *)
+    iAssert (
+        ⌜b = true⌝ -∗
+        ∀ id, ⌜o = Some id⌝ -∗
+        ∀ i_s i_t L_s L_t,
+          frame_src i_s L_s -∗
+          frame_tgt i_t L_t -∗
+          ∃ ptr v_t v_s,
+            dval_rel v_t v_s ∗
+            [ id := dvalue_to_uvalue v_t ]t i_t ∗
+            [ a := UVALUE_Addr (ptr,0)%Z ]s i_s ∗
+            ptr ↦s v_s ∗
+            frame_tgt i_t L_t ∗
+            frame_src i_s L_s)%I as "H".
+    { iIntros (?); subst; done. }
+    clear Heqb.
+
+    iInduction c as [ | ] "IH" forall (o b) "H"; eauto; cbn.
+    destruct (las_instr a o a0) eqn: Hlas.
+    destruct p.
+    cbn. iSplitR ""; cycle 1.
+    { assert (code_WF c).
+      { apply code_WF_cons_inv in H0; destruct H0; eauto. }
+      iApply ("IH" $! H1 _). iModIntro.
+      admit. }
+
+    iClear "IH".
+    destruct p, a0, b;
+    (* Not allocated yet; trivial by reflexivity, since nothing changed *)
+      [ | las_trivial Hlas].
+
+    iSpecialize ("H" $! eq_refl).
+    iIntros (????); cbn in Hlas; las_trivial Hlas.
+
+    (* Load case *)
+    clear H1 H3 H4 H5 H6 H7 H8; destructb.
+    iIntros "CI". destruct_code_inv.
+    destruct_local_inv. destruct_frame.
+    iDestruct ("H" $! _ eq_refl with "Hfs Hft") as
+      (???) "(#Hdv & Hl & Hid & Hptr & Hf_t & Hf_s)".
+
+    (* TODO: Move *)
+    assert (is_supported t) by admit.
+    assert (dvalue_has_dtyp v_s t) by admit.
+    assert (id ∉ (list_to_set args_s.*1 : gset _)). { admit. }
+    assert (id ∉ (list_to_set args_t.*1 : gset _)). { admit. }
+    iApply source_red_sim_expr.
+    do 2 destruct_frame.
+    iApply (source_red_mono with "[Hd_t Hs_t CI HL AI Hl]"); cycle 1.
+    { iApply (source_instr_load _ _ _ _ _ _ _ _ _ _ _
+                (fun x => ⌜x = Ret tt⌝ ∗
+              [ id1 := UVALUE_Addr (ptr, 0%Z) ]s i_s ∗
+              [ id := v_s ̂ ]s i_s ∗
+              ptr ↦s v_s ∗
+              ldomain_src i_s ({[id]} ∪ list_to_set args_s.*1) ∗ stack_src i_s)%I
+               with "Hptr Hid Hd_s Hs_s"); eauto.
+      iIntros "H1 Hv Hp Hd Hs". by iFrame. }
+
+    iIntros (?) "H'".
+    iDestruct "H'" as (?) "(Hid1 & Hid & Hptr & Hd & Hs)".
+
+    iApply target_red_sim_expr.
+    iApply (target_red_mono with "[CI HL AI Hid1 Hid Hptr Hd Hs]"); cycle 1.
+    { iApply (target_instr_pure with "Hs_t Hd_t [Hl]"); eauto.
+      { iIntros "Hdt Hst".
+        iApply (target_local_id with "Hst Hl").
+        iIntros "Hst Hr"; sfinal. }
+      iIntros "Hid Hd Hs". Unshelve.
+      2 : exact (fun x => ⌜x = Ret tt⌝ ∗
+                   [ id := v_t ̂ ]t i_t ∗
+                   ldomain_tgt i_t ({[id]} ∪ list_to_set args_t.*1) ∗
+                   stack_tgt i_t)%I.
+      by iFrame. }
+
+    iIntros (?) "Hf".
+    iDestruct "Hf" as (?) "(Hid1' & Hdt & Hst)"; iFrame. subst.
+    Base. sfinal. iExists ∅, ∅; sfinal.
+
+    (* Extended local environment, like the alloca environment. *)
   Admitted.
 
   Lemma las_simulation_term a b:
     term_WF (blk_term b) ->
     ⊢ term_logrel
-        (local_bij_except_promotable a)
+        local_bij
         alloca_bij
         (blk_term (las_block a None b))
         (blk_term b)
         ∅.
   Proof.
-    (* TODO: Show reflexivity of [except] for terminators, analogous to
-            expressions. *)
-  Admitted.
+    iIntros (?); iApply term_logrel_refl.
+  Qed.
 
   Lemma las_simulation_phis a be b A_t A_s :
     (blk_phis b).*1 ## (a :: nil) ->
     ⊢ phis_logrel
-        (local_bij_except [a] [a]) alloca_bij
+        local_bij alloca_bij
         be be
         (blk_phis (las_block a None b))
         (blk_phis b)
@@ -392,24 +556,18 @@ Section las_example_proof.
 
     destruct a0; iApply phi_compat; destruct p.
     destruct (Util.assoc be args) eqn: Hlu; eauto.
-    (* TODO: EASY, but tedius.
-        [expr_logrel] with [local_bij_except]. *)
-    (* TODO: Might need to strengthen
-        Propagate from [find_promotable_alloca] that we have
-        a disjoint set. *)
-    (* TODO: Not sure
-        [local_bij_except] does not include the subpredicates
-        of [local_bij_except_promotable]. *)
-  Admitted.
+    iApply expr_logrel_refl.
+  Qed.
 
   Lemma las_simulation_cfg (f : cfg dtyp) a i A_t A_s:
     cfg_WF f ->
+    (* The promotable location is not a local id that appears in the phi nodes. *)
+    (∀ b, b ∈ blks f -> ((blk_phis b).*1 ## a :: nil)) ->
+    (* Promotable location is found. *)
     find_promotable_alloca f = Some (IId a, i) ->
-    ⊢ cfg_logrel
-        (local_bij_except_promotable a)
-        alloca_bij (las f) f ∅ A_t A_s.
+    ⊢ cfg_logrel local_bij alloca_bij (las f) f ∅ A_t A_s.
   Proof.
-    intros Hwf Halloc.
+    intros Hwf Hnophi Halloc.
     iApply cfg_compat; eauto;
       [ by apply las_cfg_WF | by rewrite /las Halloc | ].
 
@@ -426,7 +584,8 @@ Section las_example_proof.
     { (* Inductive case can be trivially discharged *)
       iApply "IH"; iPureIntro; eauto.
       (* Well-formedness. *)
-      apply cfg_WF_inv in Hwf; cbn in *; by destructb. }
+      - apply cfg_WF_inv in Hwf; cbn in *; by destructb.
+      - intros; eapply Hnophi; set_solver. }
 
     iSplitL ""; first done; iIntros (???); iClear "IH".
 
@@ -438,20 +597,19 @@ Section las_example_proof.
     iApply block_compat; eauto; [ by apply las_block_WF | .. ].
 
     (* Phis logrel *)
-    { admit. }
-      (* iApply las_simulation_phis. *)
+    { iApply las_simulation_phis; set_solver. }
 
     (* Code logrel *)
     { by iApply las_simulation_code. }
 
     (* Term logrel *)
     { by iApply las_simulation_term. }
-
-  Admitted.
+  Qed.
 
   Lemma las_simulation (f : function) :
+    SSA_function f ->
     fun_WF f ->
-    ⊢ fun_logrel (las_fun f) f ∅.
+    ⊢ fun_logrel attr_inv nil (las_fun f) f ∅.
   Proof.
     iIntros; rewrite /las_fun /las; cbn.
 
@@ -468,12 +626,11 @@ Section las_example_proof.
     (* Renaming variables. *)
     rename i0 into promotable_alloca_instr.
     rename id into promotable.
-    rename H0 into fun_WF_src.
+    rename H0 into SSA_f.
+    rename H1 into fun_WF_src.
 
     (* Use compatibility of functions *)
-    iApply
-      (fun_compat
-        (local_bij_except_promotable promotable));
+    iApply (fun_compat local_bij);
       eauto; cycle 3.
 
     (* Well-formedness is maintained by the [las] transformation. *)
@@ -481,9 +638,9 @@ Section las_example_proof.
       by rewrite /las_fun /las Promotable_found in fun_WF_src. }
 
     (* State the invariant first. *)
-    { cbn; iIntros (??????) "Hlt Hls Hargs".
-      iApply local_bij_implies_local_bij_except_promotable;
-        rewrite /local_bij; iFrame.
+    { cbn; iIntros (??????) "Hlt Hls Hargs". iFrame.
+      (* iApply local_bij_implies_local_bij_except_promotable; *)
+      (*   rewrite /local_bij; iFrame. *)
       rewrite -H0; done. }
 
     (* CFG's are related to each other. *)
@@ -491,6 +648,7 @@ Section las_example_proof.
     iPoseProof (las_simulation_cfg (df_instrs f)) as "H";
       eauto; last first.
     { by rewrite /las Promotable_found. }
+    { eapply SSA_fun_implies_promotable_phi_disjoint; eauto. }
     apply fun_WF_inv in fun_WF_src; eauto.
   Qed.
 
