theories/vir/logrel/fundamental_exp_relaxed_except.v
@@ -1,0 +1,674 @@
+From iris.prelude Require Import options.
+
+From velliris.vir.lang Require Import lang.
+From velliris.vir.rules Require Import rules.
+From velliris.vir.logrel Require Import logical_relations.
+
+Set Default Proof Using "Type*".
+
+Import ListNotations.
+Import SemNotations.
+Import LLVMAst.
+
+(** *Reflexivity theorems for logical relations *)
+Section fundamental_exp.
+
+  Context {Σ : gFunctors} `{!vellirisGS Σ}.
+
+  Ltac exp_logrel_pre d :=
+    destruct d; try iApply exp_conv_raise.
+
+  Ltac exp_logrel_ret :=
+    setoid_rewrite interp_ret; iApply sim_expr_base; iExists _, _; iFrame;
+    iSplitL ""; [ | iSplitL ""]; try (iPureIntro; reflexivity);
+      iApply uval_rel_lift; eauto;
+      rewrite unfold_dval_rel; auto.
+
+  Ltac exp_logrel_num dt d :=
+    exp_logrel_pre dt; exp_logrel_pre d; exp_logrel_ret;
+    iExists _, _; do 2 (iSplitL ""; [ by iPureIntro | ]);
+      cbn; eauto.
+
+  (* ------------------------------------------------------------------------ *)
+
+  Lemma expr_logrel_EXP_Ident :
+    forall (id : LLVMAst.ident) (dt : option dtyp) i_t i_s L_t L_s,
+      local_bij_at_exp (EXP_Ident id) (EXP_Ident id : exp uvalue) i_t i_s L_t L_s
+      -∗
+      exp_conv (denote_exp dt (EXP_Ident id)) ⪯
+      exp_conv (denote_exp dt (EXP_Ident id))
+      [{ (v_t, v_s),
+          uval_rel v_t v_s ∗
+      local_bij_at_exp (EXP_Ident id) (EXP_Ident id : exp uvalue) i_t i_s L_t L_s }].
+  Proof with vsimp.
+    iIntros (id dt i_t i_s L_t L_s) "HC"; cbn.
+    rewrite /lookup_id; destruct id; cbn.
+    { (* Global *)
+      rewrite /exp_conv interp_translate interp_bind interp_vis.
+      vsimp. Cut...
+      iApply sim_expr_vis.
+      mono: iApply sim_global_read with "[HC]"...
+      final...
+      iApply sim_expr_base... vsimp.
+      rewrite !bind_tau. Tau...
+      do 2 (rewrite !interp_ret; vsimp).
+      vfinal.
+      iApply (dval_rel_lift with "HΦ"). }
+    { (* Local *)
+      rewrite /exp_conv.
+
+      rewrite interp_translate interp_vis.
+      setoid_rewrite InterpFacts.interp_ret.
+      rewrite bind_trigger.
+      iApply sim_expr_vis; rewrite !subevent_subevent.
+
+   (*    iDestruct (expr_inv_local_env_includes id with "HC") as %(Ht & Hs); *)
+   (*    [ set_solver | set_solver | ]. *)
+
+   (*    iApply sim_expr_bupd_mono ; *)
+   (*      [ | iApply (expr_local_read_refl with "HC")]; eauto; cycle 1. *)
+   (*    { cbn; case_decide; set_solver. } *)
+   (*    iIntros (??) "H". *)
+   (*    iDestruct "H" as (????) "H". *)
+   (*    rewrite H H0. rewrite !bind_ret_l. *)
+   (*    iApply sim_expr_tau; iApply sim_expr_base. *)
+   (*    iExists _, _; by iFrame. } *)
+   (* Qed. *)
+  Admitted.
+
+  Lemma expr_logrel_EXP_Integer:
+    ∀ (x : int) (dt : option dtyp),
+      ⊢ exp_conv (denote_exp dt (EXP_Integer x))
+        ⪯ exp_conv (denote_exp dt (EXP_Integer x))
+      [{ (v_t, v_s), uval_rel v_t v_s }].
+  Proof.
+    iIntros (x dt).
+    exp_logrel_pre dt. exp_logrel_pre d.
+    rewrite /denote_exp /lift_undef_or_err.
+    destruct (Functor.fmap dvalue_to_uvalue (coerce_integer_to_int sz x)) eqn: Hx;
+      destruct unEitherT, s;
+      [iApply exp_conv_raiseUB
+      | iApply exp_conv_raiseUB
+      | iApply exp_conv_raise | ].
+    setoid_rewrite interp_ret. iApply sim_expr_base; iExists _, _; iFrame.
+    iSplitL ""; [ | iSplitL ""]; try (iPureIntro; reflexivity).
+    inversion Hx.
+    destruct (EitherMonad.unEitherT (coerce_integer_to_int sz x));
+      destruct s; inversion H0; clear H0; subst.
+
+    assert (sz = 1%N \/ sz = 8%N \/ sz = 32%N \/ sz = 64%N).
+    { destruct sz; inversion Hx; destruct p; cbn in H0; inversion H0.
+      - repeat (destruct p; inversion H1); tauto.
+      - tauto. }
+    destruct H as [H | [H | [H | H ] ] ]; subst; cbn in Hx; inversion Hx;
+      iApply uval_rel_lift; eauto;
+      rewrite unfold_dval_rel; cbn; subst; eauto.
+    Unshelve. all : try eauto.
+  Qed.
+
+  Lemma expr_logrel_EXP_Float:
+    ∀ x (dt : option dtyp),
+      ⊢ exp_conv (denote_exp dt (EXP_Float x))
+        ⪯ exp_conv (denote_exp dt (EXP_Float x))
+      [{ (v_t, v_s),uval_rel v_t v_s }].
+  Proof.
+    iIntros (??); exp_logrel_num dt d.
+  Qed.
+
+  Lemma expr_logrel_EXP_Hex:
+    ∀ x (dt : option dtyp),
+      ⊢ exp_conv (denote_exp dt (EXP_Hex x))
+        ⪯ exp_conv (denote_exp dt (EXP_Hex x))
+      [{ (v_t, v_s), uval_rel v_t v_s }].
+  Proof.
+    iIntros (??); exp_logrel_num dt d.
+  Qed.
+
+  Lemma expr_logrel_EXP_Double:
+    ∀ x (dt : option dtyp),
+      ⊢ exp_conv (denote_exp dt (EXP_Double x))
+        ⪯ exp_conv (denote_exp dt (EXP_Double x))
+      [{ (v_t, v_s),uval_rel v_t v_s }].
+  Proof.
+    iIntros (??); exp_logrel_num dt d.
+  Qed.
+
+  Lemma expr_logrel_EXP_Bool:
+    ∀ x (dt : option dtyp),
+      ⊢ exp_conv (denote_exp dt (EXP_Bool x))
+        ⪯ exp_conv (denote_exp dt (EXP_Bool x))
+      [{ (v_t, v_s),uval_rel v_t v_s }].
+  Proof.
+    iIntros (b?).
+    exp_logrel_pre b; exp_logrel_ret.
+  Qed.
+
+  (* [Binop]-y operations *)
+
+  (* [OP_IBinop] *)
+  Lemma expr_logrel_OP_IBinop:
+    ∀ I (iop : ibinop) (t : dtyp) (e1 e2 : exp dtyp) (dt : option dtyp)
+      i_t i_s L_t L_s,
+      □ (∀ (a : option dtyp),
+           I i_t i_s L_t L_s e1 e1 -∗
+          exp_conv (denote_exp a e1) ⪯
+          exp_conv (denote_exp a e1)
+          [{ (v_t, v_s),
+              uval_rel v_t v_s ∗
+              code_inv I i_t i_s L_t L_s e1 e1 }]) -∗
+        (∀ (a : option dtyp),
+          code_inv I i_t i_s L_t L_s e2 e2 -∗
+          exp_conv (denote_exp a e2) ⪯
+          exp_conv (denote_exp a e2)
+          [{ (v_t, v_s),
+              uval_rel v_t v_s ∗
+              code_inv I i_t i_s L_t L_s e2 e2  }]) -∗
+        code_inv I i_t i_s L_t L_s
+          (OP_IBinop iop t e1 e2)
+          (OP_IBinop iop t e1 e2)  -∗
+        exp_conv (denote_exp dt (OP_IBinop iop t e1 e2)) ⪯
+        exp_conv (denote_exp dt (OP_IBinop iop t e1 e2))
+      [{ (v_t, v_s),
+          uval_rel v_t v_s ∗
+          expr_inv i_t i_s L_t L_s
+            (OP_IBinop iop t e1 e2)
+            (OP_IBinop iop t e1 e2) }].
+  Proof.
+    iIntros (iop t e1 e2 dt ????) "#IH IH1 HI".
+
+    iDestruct (expr_inv_binop_invert with "HI") as "(HI&H2)".
+
+    iSpecialize ("IH" $! (Some t) with "HI").
+    cbn; setoid_rewrite interp_bind.
+    iApply sim_expr_bind.
+    iApply (sim_expr_bupd_mono with "[IH1 H2]"); [ | iApply "IH"].
+    iIntros (e_t e_s) "H".
+    iDestruct "H" as (?? Ht Hs) "(Hv & HI)".
+    rename v_t into v1', v_s into v1.
+    rewrite Ht Hs; clear Ht Hs.
+    do 2 rewrite bind_ret_l interp_bind.
+
+    iDestruct (expr_local_env_inv_commute with "HI H2") as "(HI & H1)".
+
+    iSpecialize ("IH1" $! (Some t) with "HI").
+    iApply sim_expr_bind.
+    iApply (sim_expr_bupd_mono with "[H1 Hv]"); [ | iApply "IH1"].
+    clear e_t e_s.
+    iIntros (e_t e_s) "H".
+    iDestruct "H" as (?? Ht Hs) "(Hv0 & HI)".
+    rewrite Ht Hs; clear Ht Hs.
+    do 2 rewrite bind_ret_l. subst.
+    rename v_t into v2', v_s into v2.
+
+    do 2 rewrite interp_ret. iApply sim_expr_base.
+    do 2 iExists _. do 2 (iSplitL ""; [ done | ]).
+    iSplitL "Hv Hv0"; first iApply (uval_rel_binop with "Hv Hv0").
+    iApply expr_inv_binop; iFrame.
+    iApply (expr_local_env_inv_commute with "HI H1").
+  Qed.
+
+  (* [OP_ICmp]*)
+  Lemma expr_logrel_OP_ICmp:
+    ∀ iop (t : dtyp) (e1 e2 : exp dtyp) (dt : option dtyp)
+      i_t i_s L_t L_s,
+      □ (∀ (a : option dtyp),
+          expr_inv i_t i_s L_t L_s e1 e1 -∗
+          exp_conv (denote_exp a e1) ⪯
+          exp_conv (denote_exp a e1)
+          [{ (v_t, v_s),
+              uval_rel v_t v_s ∗
+              expr_inv i_t i_s L_t L_s e1 e1 }]) -∗
+        (∀ (a : option dtyp),
+          expr_inv i_t i_s L_t L_s e2 e2 -∗
+          exp_conv (denote_exp a e2) ⪯
+          exp_conv (denote_exp a e2)
+          [{ (v_t, v_s),
+              uval_rel v_t v_s ∗
+              expr_inv i_t i_s L_t L_s e2 e2  }]) -∗
+        expr_inv i_t i_s L_t L_s
+          (OP_ICmp iop t e1 e2)
+          (OP_ICmp iop t e1 e2)  -∗
+        exp_conv (denote_exp dt (OP_ICmp iop t e1 e2)) ⪯
+        exp_conv (denote_exp dt (OP_ICmp iop t e1 e2))
+      [{ (v_t, v_s),
+          uval_rel v_t v_s ∗
+          expr_inv i_t i_s L_t L_s
+            (OP_ICmp iop t e1 e2)
+            (OP_ICmp iop t e1 e2) }].
+  Proof.
+    iIntros (iop t e1 e2 dt ????) "#IH IH1 HI".
+
+    iDestruct (expr_inv_icmp_invert with "HI") as "(HI&H2)".
+
+    iSpecialize ("IH" $! (Some t) with "HI").
+    cbn; setoid_rewrite interp_bind.
+    iApply sim_expr_bind.
+    iApply (sim_expr_bupd_mono with "[IH1 H2]"); [ | iApply "IH"].
+    iIntros (e_t e_s) "H".
+    iDestruct "H" as (?? Ht Hs) "(Hv & HI)".
+    rename v_t into v1', v_s into v1.
+    rewrite Ht Hs; clear Ht Hs.
+    do 2 rewrite bind_ret_l interp_bind.
+
+    iDestruct (expr_local_env_inv_commute with "HI H2") as "(HI & H1)".
+
+    iSpecialize ("IH1" $! (Some t) with "HI").
+    iApply sim_expr_bind.
+    iApply (sim_expr_bupd_mono with "[H1 Hv]"); [ | iApply "IH1"].
+    clear e_t e_s.
+    iIntros (e_t e_s) "H".
+    iDestruct "H" as (?? Ht Hs) "(Hv0 & HI)".
+    rewrite Ht Hs; clear Ht Hs.
+    do 2 rewrite bind_ret_l. subst.
+    rename v_t into v2', v_s into v2.
+
+    do 2 rewrite interp_ret. iApply sim_expr_base.
+    do 2 iExists _. do 2 (iSplitL ""; [ done | ]).
+    iSplitL "Hv Hv0"; first iApply (uval_rel_icmp with "Hv Hv0").
+    iApply expr_inv_icmp; iFrame.
+    iApply (expr_local_env_inv_commute with "HI H1").
+  Qed.
+
+  Tactic Notation "expr_case" constr(lem) :=
+    iApply (sim_expr_mono with "[HI]"); last iApply lem;
+        eauto;
+      iIntros (??) "H"; iDestruct "H" as (????) "Hv";
+      iExists _, _; by iFrame.
+
+  (* Inductive cases *)
+
+  (* TODO: Factor out the [expr_inv] into an arbitrary invariant *)
+   Lemma expr_logrel_ind_case :
+     forall (elts : list (dtyp * exp dtyp)) i_t i_s L_t L_s Vexp (Exp : _ -> exp dtyp),
+    (* [uval_rel] nil case *)
+    □ (uval_rel (Vexp []) (Vexp [])) -∗
+    (* [uval_rel] cons case *)
+    □ (∀ v_t v_s l_t l_s,
+      uval_rel v_t v_s -∗
+      uval_rel (Vexp l_t) (Vexp l_s) -∗
+      uval_rel (Vexp (v_t :: l_t)) (Vexp (v_s :: l_s))) -∗
+    (* [expr_inv] cons over the struct values *)
+    □ (∀ i_t i_s L_t L_s d e elts,
+        expr_inv i_t i_s L_t L_s e e ∗
+        expr_local_env_inv i_t i_s (exp_local_ids (Exp elts)) L_t L_s
+        ∗-∗
+        expr_inv i_t i_s L_t L_s (Exp ((d, e) :: elts)) (Exp ((d, e) :: elts))) -∗
+    (* [expr_inv] introduction over the struct values *)
+    □ (∀ i_t i_s L_t L_s elts,
+      expr_inv i_t i_s L_t L_s (Exp elts) (Exp elts) -∗
+       expr_frame_inv i_t i_s L_t L_s ∗
+        (∀ x, ⌜In x elts⌝ -∗
+          expr_local_env_inv i_t i_s (exp_local_ids x.2) L_t L_s)) -∗
+    □ (∀ x : dtyp * exp dtyp,
+      ⌜In x elts⌝
+      → ∀ (a : option dtyp) i_t i_s L_t L_s,
+          expr_inv i_t i_s L_t L_s x.2 x.2 -∗
+            exp_conv (denote_exp a x.2) ⪯
+            exp_conv (denote_exp a x.2)
+            [{ (v_t, v_s),
+                uval_rel v_t v_s ∗ expr_inv i_t i_s L_t L_s x.2 x.2 }]) -∗
+      expr_inv i_t i_s L_t L_s (Exp elts) (Exp elts) -∗
+      r <- exp_conv
+            (map_monad (λ '(dt0, ex), (denote_exp (Some dt0) ex)) elts);;
+      Ret (Vexp r)
+      ⪯
+      r <-  exp_conv (map_monad (λ '(dt0, ex), (denote_exp (Some dt0) ex)) elts);;
+      Ret (Vexp r)
+    [{ (v_t, v_s),
+        uval_rel v_t v_s ∗
+          expr_inv i_t i_s L_t L_s (Exp elts) (Exp elts) }].
+  Proof.
+    iIntros (elts i_t i_s L_t L_s Vexp Exp) "#Hbase #Hind #Hinv #Hinvp #IH HI".
+    rewrite /exp_conv.
+    (* We follow by induction on the structure elements. *)
+    iInduction elts as [] "IHl".
+    (* nil case *)
+    { cbn; rewrite interp_ret bind_ret_l.
+      iApply sim_expr_base; iExists _, _; iFrame;
+      iSplitL ""; [ | iSplitL ""]; try (iPureIntro; reflexivity); done. }
+    (* cons case *)
+    { cbn. destruct a. rewrite /exp_conv.
+      rewrite interp_bind bind_bind.
+      iApply sim_expr_bind.
+
+      iDestruct ("Hinv" with "HI") as "(He & Helts)".
+
+      iSpecialize ("IHl" with "[]").
+      { iModIntro. iIntros (x Hin dt' i_t' i_s' L_t' L_s') "Hinv'".
+        assert ((d, e) = x \/ In x elts) by (by right).
+        by iSpecialize ("IH" $! _ H dt' i_t' i_s' L_t' L_s' with "Hinv'"). }
+
+      assert (EQ: (d, e) = (d, e) ∨ In (d, e) elts) by (left; auto).
+      iSpecialize ("IH" $! (d, e) EQ _ _); clear EQ; cbn.
+      iSpecialize ("IH" with "He").
+      iApply (sim_expr_bupd_mono with "[Helts]"); [ | done].
+      iIntros (??) "Hr".
+      iDestruct "Hr" as (????) "[Hv Hinv']".
+      rewrite H H0. do 2 rewrite bind_ret_l.
+      iDestruct (expr_local_env_inv_commute with "Hinv' Helts") as "(Helts & Hinv')".
+      iSpecialize ("IHl" with "Helts"). iModIntro.
+      do 2 rewrite interp_bind bind_bind.
+      setoid_rewrite interp_ret.
+      setoid_rewrite bind_ret_l.
+      iPoseProof sim_expr_fmap_inv as "Hfmap".
+      iSpecialize ("Hfmap" with "IHl").
+      iApply sim_expr_bind.
+      iApply (sim_expr_bupd_mono with "[Hinv' Hv]"); [ | done].
+      iIntros (??) "Hp". rewrite /lift_post.
+      iDestruct "Hp" as (????????) "[Hp CI]".
+      apply eqit_inv_Ret in H3, H4; subst. rewrite H1 H2. do 2 rewrite bind_ret_l.
+      iApply sim_expr_base. iModIntro; do 2 iExists _. eauto.
+      iSplitL ""; [| iSplitL ""]; auto; iFrame.
+      iSplitL "Hv Hp"; first iApply ("Hind" with "Hv Hp").
+      iApply "Hinv"; iFrame.
+      iApply (expr_local_env_inv_commute with "CI Hinv'"). }
+  Qed.
+
+  Lemma expr_logrel_EXP_Cstring:
+    ∀ (elts : list (dtyp * exp dtyp))
+      (τ : option dtyp) (i_t i_s : list frame_names) (L_t L_s : local_env),
+    expr_inv i_t i_s L_t L_s (EXP_Cstring elts) (EXP_Cstring elts) -∗
+    □ (∀ x : dtyp * exp dtyp,
+        ⌜In x elts⌝
+        → ∀ (τ0 : option dtyp) (i_t0 i_s0 : list frame_names) (L_t0 L_s0 : local_env),
+            expr_inv i_t0 i_s0 L_t0 L_s0 x.2 x.2 -∗
+            exp_conv (denote_exp τ0 x.2)
+            ⪯
+            exp_conv (denote_exp τ0 x.2)
+            [{ (v_t, v_s),uval_rel v_t v_s ∗ expr_inv i_t0 i_s0 L_t0 L_s0 x.2 x.2}]) -∗
+    exp_conv (denote_exp τ (EXP_Cstring elts))
+    ⪯
+    exp_conv (denote_exp τ (EXP_Cstring elts))
+    [{ (v_t, v_s),
+        uval_rel v_t v_s ∗
+          expr_inv i_t i_s L_t L_s (EXP_Cstring elts) (EXP_Cstring elts)}].
+  Proof.
+    intros elts dt ? ? ? ?. iIntros "Hi #IH".
+    cbn; setoid_rewrite interp_bind; setoid_rewrite interp_ret.
+    iApply expr_logrel_ind_case; auto.
+    { iModIntro; cbn; iApply uval_rel_lift; eauto;
+        rewrite unfold_dval_rel; auto. cbn; done. }
+    { iModIntro.
+      iIntros (v_t v_s l_t l_s) "Hv Hl".
+      iApply (uval_rel_array_cons with "Hv Hl"); cbn; iFrame. }
+    { iModIntro. iIntros. iApply expr_inv_cstring_cons. }
+    { iModIntro. iIntros. by iApply expr_inv_cstring_invert. }
+  Qed.
+
+  Lemma expr_logrel_EXP_Struct:
+    ∀ (fields : list (dtyp * exp dtyp))
+      (τ : option dtyp)
+      (i_t i_s : list frame_names) (L_t L_s : local_env),
+      expr_inv i_t i_s L_t L_s
+        (EXP_Struct fields) (EXP_Struct fields) -∗
+      □ (∀ x : dtyp * exp dtyp,
+          ⌜In x fields⌝
+          → ∀ (τ0 : option dtyp) (i_t0 i_s0 : list frame_names) (L_t0 L_s0 : local_env),
+              expr_inv i_t0 i_s0 L_t0 L_s0 x.2 x.2 -∗
+              exp_conv (denote_exp τ0 x.2)
+              ⪯
+              exp_conv (denote_exp τ0 x.2)
+              [{ (v_t, v_s), uval_rel v_t v_s ∗ expr_inv i_t0 i_s0 L_t0 L_s0 x.2 x.2}]) -∗
+      exp_conv (denote_exp τ (EXP_Struct fields))
+      ⪯
+      exp_conv (denote_exp τ (EXP_Struct fields))
+      [{ (v_t, v_s), uval_rel v_t v_s ∗
+            expr_inv i_t i_s L_t L_s (EXP_Struct fields) (EXP_Struct fields)}].
+  Proof.
+    intros elts dt ? ? ? ?. iIntros "Hi #IH".
+    cbn; setoid_rewrite interp_bind; setoid_rewrite interp_ret.
+    iApply expr_logrel_ind_case; auto.
+    { iModIntro; cbn; iApply uval_rel_lift; eauto;
+        rewrite unfold_dval_rel; auto. cbn; done. }
+    { iModIntro.
+      iIntros (v_t v_s l_t l_s) "Hv Hl".
+      iApply (uval_rel_struct_cons with "Hv Hl"); cbn; iFrame. }
+    { iModIntro. iIntros. iApply expr_inv_struct_cons. }
+    { iModIntro. iIntros. by iApply expr_inv_struct_invert. }
+  Qed.
+
+  Lemma expr_logrel_OP_Conversion:
+    ∀ (conv : conversion_type)
+      (t_from t_to : dtyp)
+      (e : exp dtyp)
+      (τ : option dtyp)
+      (i_t i_s : list frame_names)
+      (L_t L_s : local_env),
+      expr_inv i_t i_s L_t L_s
+        (OP_Conversion conv t_from e t_to)
+        (OP_Conversion conv t_from e t_to) -∗
+      □ (∀ (τ0 : option dtyp) (i_t0 i_s0 : list frame_names) (L_t0 L_s0 : local_env),
+          expr_inv i_t0 i_s0 L_t0 L_s0 e e -∗
+          exp_conv (denote_exp τ0 e)
+          ⪯
+          exp_conv (denote_exp τ0 e)
+          [{ (v_t, v_s),
+              uval_rel v_t v_s ∗
+              expr_inv i_t0 i_s0 L_t0 L_s0 e e}]) -∗
+      exp_conv (denote_exp τ (OP_Conversion conv t_from e t_to))
+      ⪯
+      exp_conv (denote_exp τ (OP_Conversion conv t_from e t_to))
+      [{ (v_t, v_s),uval_rel v_t v_s ∗
+          expr_inv i_t i_s L_t L_s
+          (OP_Conversion conv t_from e t_to) (OP_Conversion conv t_from e t_to)}].
+  Proof.
+    iIntros (?????????) "Hi #IH".
+    iPoseProof (expr_inv_op_conversion with "Hi") as "Hi".
+
+    cbn.
+    cbn; setoid_rewrite interp_bind.
+    iApply sim_expr_bind.
+    iApply sim_expr_bupd_mono; [ | iApply "IH"]; try done.
+    cbn.
+    iIntros (e_t e_s) "H".
+    iDestruct "H" as (?? Ht Hs) "(Hv & HI)".
+    subst.
+    rewrite Ht Hs; clear Ht Hs.
+    do 2 rewrite bind_ret_l.
+    do 2 rewrite interp_ret. iApply sim_expr_base.
+    do 2 iExists _. do 2 (iSplitL ""; [ done | ]).
+    rewrite /uval_rel. iFrame.
+    iModIntro; iIntros (??). inversion H.
+  Qed.
+
+  Lemma expr_logrel_EXP_GEP :
+    ∀ (t : dtyp)
+      (ptrval : dtyp * exp dtyp)
+      (idxs : list (dtyp * exp dtyp))
+      (τ : option dtyp)
+      (i_t i_s : list frame_names)
+      (L_t L_s : local_env),
+    □ (∀ x : dtyp * exp dtyp,
+         ⌜In x idxs⌝ →
+        ∀ τ0 i_t0 i_s0 L_t0 L_s0,
+          expr_inv i_t0 i_s0 L_t0 L_s0 x.2 x.2 -∗
+          exp_conv (denote_exp τ0 x.2) ⪯
+          exp_conv (denote_exp τ0 x.2)
+        [{ (v_t, v_s), uval_rel v_t v_s ∗
+          expr_inv i_t0 i_s0 L_t0 L_s0 x.2 x.2}]) -∗
+    □ (∀ τ0 i_t0 i_s0 L_t0 L_s0,
+         expr_inv i_t0 i_s0 L_t0 L_s0 ptrval.2 ptrval.2 -∗
+         exp_conv (denote_exp τ0 ptrval.2) ⪯
+         exp_conv (denote_exp τ0 ptrval.2)
+        [{ (v_t, v_s), uval_rel v_t v_s ∗
+            expr_inv i_t0 i_s0 L_t0 L_s0 ptrval.2 ptrval.2}]) -∗
+      expr_inv i_t i_s L_t L_s
+        (OP_GetElementPtr t ptrval idxs)
+        (OP_GetElementPtr t ptrval idxs) -∗
+      exp_conv (denote_exp τ (OP_GetElementPtr t ptrval idxs))
+      ⪯
+      exp_conv (denote_exp τ (OP_GetElementPtr t ptrval idxs))
+      [{ (v_t, v_s), uval_rel v_t v_s ∗
+          expr_inv i_t i_s L_t L_s
+            (OP_GetElementPtr t ptrval idxs)
+            (OP_GetElementPtr t ptrval idxs) }].
+  Proof.
+    iIntros (t (ptr_t &e1) dt idxs ? ? ? ? ) "#IH1 #IH2 HI".
+
+    iDestruct (expr_inv_op_gep_invert with "HI") as "(He & HI)".
+    cbn. setoid_rewrite interp_bind.
+    iSpecialize ("IH2" with "He").
+    iApply sim_expr_bind.
+    iApply (sim_expr_bupd_mono with "[HI IH1]"); [ | iApply "IH2"].
+    iIntros (e_t e_s) "H".
+
+    iDestruct "H" as (?? Ht Hs) "(Hv & HI')".
+    rename v_t into v1', v_s into v1.
+    rewrite Ht Hs; clear Ht Hs.
+    do 2 rewrite bind_ret_l interp_bind.
+    setoid_rewrite interp_ret.
+
+    iInduction dt as [] "IHl".
+    - cbn. rewrite interp_ret bind_ret_l.
+      rewrite bind_ret_l. iApply sim_expr_base.
+      iExists (UVALUE_GetElementPtr t v1' []), (UVALUE_GetElementPtr t v1 []).
+      iModIntro. do 2 (iSplitL ""; [ done | ]).
+      iSplitL "Hv".
+      { rewrite /uval_rel; cbn.
+        iIntros (??). inversion H. }
+
+      iDestruct "HI'" as "(Hf & HI')".
+      rewrite /expr_inv; iFrame.
+      rewrite !intersection_local_ids_eq; cbn.
+      rewrite app_nil_r; done.
+
+    - cbn. destruct a. rewrite interp_bind; do 2 rewrite bind_bind.
+      iApply sim_expr_bind.
+      iSpecialize ("IHl" with "[]").
+      { iModIntro. iIntros (x Hin dt' i_t' i_s' L_t' L_s') "Hinv".
+        assert ((d, e) = x \/ In x dt) by (by right).
+        by iSpecialize ("IH1" $! _ H with "Hinv"). }
+      assert (EQ : ((d, e) = (d, e) \/ In (d, e) dt)). { by left. }
+      iSpecialize ("IH1" $! _ EQ).
+      iDestruct "HI" as "(He & HI)".
+      iDestruct (expr_local_env_inv_commute with "HI' He") as "(He & Heq)".
+      iSpecialize ("IH1" $! _ i_t i_s L_t L_s with "He").
+      iApply (sim_expr_bupd_mono with "[HI Heq Hv]"); [ | done].
+
+      iIntros (??) "Hr".
+      iDestruct "Hr" as (????) "[Hv' Hinv]".
+      rewrite H H0. do 2 rewrite bind_ret_l.
+
+      iDestruct (expr_local_env_inv_commute with "Hinv Heq") as "(He & Heq)".
+      iSpecialize ("IHl" with "HI Hv He").
+
+      do 2 rewrite interp_bind bind_bind.
+      setoid_rewrite interp_ret.
+      setoid_rewrite bind_ret_l.
+      iPoseProof sim_expr_fmap_inv as "Hfmap".
+      iMod "IHl". iSpecialize ("Hfmap" with "IHl").
+      iApply sim_expr_bind.
+      iApply (sim_expr_bupd_mono with "[Heq Hv']"); [ | done].
+      iIntros (??) "Hp". rewrite /lift_post.
+      iDestruct "Hp" as (????????) "[Hp CI]".
+      apply eqit_inv_Ret in H3, H4; subst. rewrite H1 H2. do 2 rewrite bind_ret_l.
+      iApply sim_expr_base. iModIntro; do 2 iExists _.
+      do 2 (iSplitL ""; first done).
+      iSplitL "Hv' Hp".
+      { rewrite /uval_rel; eauto. }
+
+      iDestruct (expr_inv_op_gep_invert with "CI") as "((Hf & He) & HI)";
+      rewrite /expr_inv; iFrame.
+      rewrite !intersection_local_ids_eq. cbn -[expr_local_env_inv].
+      iApply (expr_local_env_inv_app with "He"). rewrite app_nil_r.
+      iApply (expr_local_env_inv_app with "Heq").
+      by iApply expr_local_env_inv_big_opL.
+  Qed.
+
+  Lemma expr_logrel_EXP_Array:
+    ∀ (fields : list (dtyp * exp dtyp))
+      (τ : option dtyp)
+      (i_t i_s : list frame_names) (L_t L_s : local_env),
+      expr_inv i_t i_s L_t L_s
+        (EXP_Array fields) (EXP_Array fields) -∗
+      □ (∀ x : dtyp * exp dtyp,
+          ⌜In x fields⌝
+          → ∀ (τ0 : option dtyp) (i_t0 i_s0 : list frame_names) (L_t0 L_s0 : local_env),
+              expr_inv i_t0 i_s0 L_t0 L_s0 x.2 x.2 -∗
+              exp_conv (denote_exp τ0 x.2)
+              ⪯
+              exp_conv (denote_exp τ0 x.2)
+              [{ (v_t, v_s), uval_rel v_t v_s ∗ expr_inv i_t0 i_s0 L_t0 L_s0 x.2 x.2}]) -∗
+      exp_conv (denote_exp τ (EXP_Array fields))
+      ⪯
+      exp_conv (denote_exp τ (EXP_Array fields))
+      [{ (v_t, v_s), uval_rel v_t v_s ∗
+            expr_inv i_t i_s L_t L_s (EXP_Array fields) (EXP_Array fields)}].
+  Proof.
+    intros elts dt ? ? ? ?. iIntros "Hi #IH".
+    cbn; setoid_rewrite interp_bind; setoid_rewrite interp_ret.
+    iApply expr_logrel_ind_case; auto.
+    { iModIntro; cbn; iApply uval_rel_lift; eauto;
+        rewrite unfold_dval_rel; auto. cbn; done. }
+    { iModIntro.
+      iIntros (v_t v_s l_t l_s) "Hv Hl".
+      iApply (uval_rel_array_cons with "Hv Hl"); cbn; iFrame. }
+    { iModIntro. iIntros. iApply expr_inv_array_cons. }
+    { iModIntro. iIntros. by iApply expr_inv_array_invert. }
+  Qed.
+
+  (* Reflexivity theorems *)
+  Theorem expr_logrel_relaxed_refl e:
+    (⊢ expr_logrel_relaxed e e)%I.
+  Proof.
+    iIntros. rewrite /expr_logrel_relaxed.
+    iInduction e as [] "IH" using AstLib.exp_ind;
+    iIntros (τ ? ? L_t L_s) "HI".
+    { (* EXP_Ident *)
+      by iApply expr_logrel_EXP_Ident. }
+    (* Numeric cases *)
+    { iApply (sim_expr_mono with "[HI]"); last iApply expr_logrel_EXP_Integer;
+        eauto.
+      iIntros (??) "H". iDestruct "H" as (????) "Hv".
+      iExists _, _; by iFrame. }
+    { expr_case expr_logrel_EXP_Float. }
+    { expr_case expr_logrel_EXP_Double. }
+    { expr_case expr_logrel_EXP_Hex. }
+    { expr_case expr_logrel_EXP_Bool. }
+
+    { (* EXP_Null *)
+      iApply sim_null_bij. iIntros "#Hn".
+      setoid_rewrite interp_ret; iApply sim_expr_base; iExists _ , _;
+        iFrame; iSplitL ""; [  | iSplitL "" ]; try (iPureIntro; reflexivity).
+      iApply uval_rel_lift; eauto.
+      by rewrite unfold_dval_rel. }
+
+    { (* EXP_Zero_initializer *)
+      iApply sim_null_bij. iIntros "#Hn".
+      exp_logrel_pre τ. rewrite /exp_conv /denote_exp /lift_err; cbn.
+      destruct (dv_zero_initializer d) eqn: Hzi.
+      - iApply exp_conv_raise.
+      - setoid_rewrite interp_ret; iApply sim_expr_base; iExists _, _; iFrame;
+        iSplitL ""; [ | iSplitL ""]; try (iPureIntro; reflexivity).
+        iApply dval_rel_lift.
+        iApply (@zero_initializer_uval_refl _ _ _ _ Hzi with "Hn"). }
+
+    { (* EXP_CString *)
+      by iApply (expr_logrel_EXP_Cstring with "HI"). }
+
+    { (* EXP_Undef *)
+      destruct τ; cbn; [ | iApply exp_conv_raise ].
+      iApply sim_null_bij. iIntros "#Hnull".
+      setoid_rewrite interp_ret; iApply sim_expr_base; iExists _ , _;
+        iFrame; iSplitL ""; [  | iSplitL "" ]; try (iPureIntro; reflexivity).
+      by iApply uval_rel_undef. }
+
+    { by iApply (expr_logrel_EXP_Struct with "HI"). }
+
+    (* EXP_Array *)
+    { by iApply (expr_logrel_EXP_Array with "HI"). }
+
+    { iApply expr_logrel_OP_IBinop; eauto.
+      - iModIntro; iIntros; iApply "IH"; done.
+      - iIntros; iApply "IH1"; done. }
+
+    { iApply expr_logrel_OP_ICmp; eauto.
+      - iModIntro; iIntros; iApply "IH"; done.
+      - iIntros; iApply "IH1"; done. }
+
+    { by iApply (expr_logrel_OP_Conversion with "HI"). }
+
+    { iApply expr_logrel_EXP_GEP; eauto. }
+  Qed.
+
+End fundamental_exp.
